src/klas/Klas.Rot.fst
@@ -1,0 +1,34 @@
+module Klas.Rot
+
+(* See Klas.Rot.fsti for the specification. *)
+
+#lang-pulse
+open Kuiper
+open Kuiper.Array1
+open Kuiper.Tensor.Layout.Alg { l1_forward }
+module Map = Kuiper.Kernel.Map
+
+inline_for_extraction noextract
+fn rot_gen (#et:Type0) {| floating et |}
+  (c s : et)
+  (lena : szp { lena <= max_blocks * max_threads })
+  (x : array1 et (l1_forward lena) { is_global x })
+  (y : array1 et (l1_forward lena) { is_global y })
+  (#vx : erased (lseq et lena))
+  (#vy : erased (lseq et lena))
+  preserves cpu
+  requires
+    on gpu_loc (x |-> vx) ** on gpu_loc (y |-> vy)
+  ensures
+    on gpu_loc (x |-> s_rot_x c s vx vy) ** on gpu_loc (y |-> s_rot_y c s vx vy)
+{
+  let tmp = alloc0 #et lena (l1_forward lena);
+  memcpy_device_to_device tmp x lena;
+  Map.map_gpu2 (fun (xi yi : et) -> add (mul c xi) (mul s yi)) lena x y;
+  Map.map_gpu2 (fun (yi ti : et) -> sub (mul c yi) (mul s ti)) lena y tmp;
+  free tmp;
+}
+
+let rot_f16 = rot_gen #f16
+let rot_f32 = rot_gen #f32
+let rot_f64 = rot_gen #f64
